wip

LeanSubst/Ops.lean
@@ -6,21 +6,165 @@ namespace LeanSubst
 universe u1 u2 u3
 variable {S : Type u1} {T : Type u2}
 
+----------------------------------------------------------------------------------------------------
+---- Translation
+----------------------------------------------------------------------------------------------------
+def Ren.het T (r : Ren) : HetRen T := ⟨r.act⟩
+
+@[simp]
+theorem Ren.het_act {r : Ren} {x} : (r.het T).act x = r.act x := by simp [Ren.het]
+
+def HetRen.forget (r : HetRen T) : Ren := ⟨r.act⟩
+
+@[simp]
+theorem HetRen.forget_act {r : HetRen T} {x} : r.forget.act x = r.act x := by simp [HetRen.forget]
+
+@[simp]
+theorem Ren.het_forget (r : Ren) : (r.het T).forget = r := by simp [Ren.het, HetRen.forget]
+
+@[simp]
+theorem HetRen.forget_het (r : HetRen T) : r.forget.het T = r := by simp [Ren.het, HetRen.forget]
+
+def Subst.het S (σ : Subst T) : HetSubst S T := ⟨σ.act⟩
+
+@[simp]
+theorem Subst.het_act {r : Subst T} {x} : (r.het S).act x = r.act x := by simp [Subst.het]
+
+def HetSubst.forget (σ : HetSubst S T) : Subst T := ⟨σ.act⟩
+
+@[simp]
+theorem HetSubst.forget_act {r : HetSubst S T} {x} : r.forget.act x = r.act x := by
+  simp [HetSubst.forget]
+
+@[simp]
+theorem Subst.het_forget (σ : Subst T) : (σ.het S).forget = σ := by
+  simp [Subst.het, HetSubst.forget]
+
+@[simp]
+theorem HetSubst.forget_het (σ : HetSubst S T) : σ.forget.het S = σ := by
+  simp [Subst.het, HetSubst.forget]
+
+def Ren.to (r : Ren) : Subst S := ⟨λ x => re (r.act x)⟩
+
+@[simp]
+theorem Ren.to_act {r : Ren} {x} : (@Ren.to S r).act x = re (r.act x) := by simp [Ren.to]
+
+def HetRen.to (r : HetRen T) : HetSubst S T := ⟨λ x => re (r.act x)⟩
+
+@[simp]
+theorem HetRen.to_act {r : HetRen T} {x} : (@HetRen.to S T r).act x = re (r.act x) := by
+  simp [HetRen.to]
+----------------------------------------------------------------------------------------------------
+---- Action
+----------------------------------------------------------------------------------------------------
+@[simp]
+def Action.rmap [RenMap S] (r : Ren) : Action S -> Action S
+| re x => re $ r.act x
+| su t => su t⟨r⟩
+
+instance [RenMap S] : RenMap (Action S) where
+  rmap := Action.rmap
+
+@[simp]
+theorem Action.rmap_re [RenMap S] {r : Ren} {x : Nat}
+  : (@re S x)⟨r⟩ = re (r.act x)
+:= by simp [RenMap.rmap]
+
+@[simp]
+theorem Action.rmap_su [RenMap S] {r : Ren} {t : S} : (su t)⟨r⟩ = su t⟨r⟩ := by simp [RenMap.rmap]
+
+@[simp]
+def Action.hsmap [SubstMap S] (σ : HetSubst (Action S) S) : Action S -> Action S
+| re x => σ.act x
+| su t => su t[σ.forget]
+
+instance [SubstMap S] : HetSubstMap (Action S) S where
+  hsmap := Action.hsmap
+
+@[simp]
+theorem Action.hsmap_re [SubstMap S] {σ : HetSubst (Action S) S} {x : Nat}
+  : (@re S x)[σ] = σ.act x
+:= by simp [HetSubstMap.hsmap]
+
+@[simp]
+theorem Action.hsmap_su [SubstMap S] {σ : HetSubst (Action S) S} {t : S}
+  : (su t)[σ] = su t[σ.forget]
+:= by simp [HetSubstMap.hsmap]
+----------------------------------------------------------------------------------------------------
+---- Identity
+----------------------------------------------------------------------------------------------------
 def Ren.id : Ren := ⟨λ x => x⟩
 
 @[simp]
 theorem Ren.id_action {x} : id.act x = x := by simp [Ren.id]
 
+def HetRen.id T : HetRen T := ⟨λ x => x⟩
+
+@[simp]
+theorem HetRen.id_action {x} : (id T).act x = x := by simp [HetRen.id]
+
+def Subst.id : Subst S := ⟨λ x => re x⟩
+notation "+0" => Subst.id
+
+@[simp]
+theorem Subst.id_action {x} : (@id S).act x = re x := by simp [Subst.id]
+
+def HetSubst.id T : HetSubst S T := ⟨λ x => re x⟩
+macro "+0@" noWs T:term : term =>`(HetSubst.id $T)
+
+@[simp]
+theorem HetSubst.id_action {x} : (@id S T).act x = re x := by simp [HetSubst.id]
+----------------------------------------------------------------------------------------------------
+---- Successor
+----------------------------------------------------------------------------------------------------
 def Ren.succ : Ren := ⟨(· + 1)⟩
 
 @[simp]
 theorem Ren.succ_action {x} : succ.act x = x + 1 := by simp [Ren.succ]
 
+def HetRen.succ T : HetRen T := ⟨(· + 1)⟩
+
+@[simp]
+theorem HetRen.succ_action {x} : (succ T).act x = x + 1 := by simp [HetRen.succ]
+
+def Subst.succ : Subst S := ⟨λ x => re $ x + 1⟩
+notation "+1" => Subst.succ
+
+@[simp]
+theorem Subst.succ_action {x} : (@succ S).act x = re (x + 1) := by simp [Subst.succ]
+
+def HetSubst.succ T : HetSubst S T := ⟨λ x => re $ x + 1⟩
+macro "+1@" noWs T:term : term =>`(HetSubst.succ $T)
+
+@[simp]
+theorem HetSubst.succ_action {x} : (@succ S T).act x = re (x + 1) := by simp [HetSubst.succ]
+----------------------------------------------------------------------------------------------------
+---- Predecessor
+----------------------------------------------------------------------------------------------------
 def Ren.pred : Ren := ⟨(· - 1)⟩
 
 @[simp]
 theorem Ren.pred_action {x} : pred.act x = x - 1 := by simp [Ren.pred]
 
+def HetRen.pred T : HetRen T := ⟨(· - 1)⟩
+
+@[simp]
+theorem HetRen.pred_action {x} : (pred T).act x = x - 1 := by simp [HetRen.pred]
+
+def Subst.pred : Subst S := ⟨λ x => re $ x - 1⟩
+notation "-1" => Subst.pred
+
+@[simp]
+theorem Subst.pred_action {x} : (@pred S).act x = re (x - 1) := by simp [Subst.pred]
+
+def HetSubst.pred : HetSubst S T := ⟨λ x => re $ x - 1⟩
+macro "-1@" noWs T:term : term =>`(HetSubst.pred $T)
+
+@[simp]
+theorem HetSubst.pred_action {x} : (@pred S T).act x = re (x - 1) := by simp [HetSubst.pred]
+----------------------------------------------------------------------------------------------------
+---- Addition
+----------------------------------------------------------------------------------------------------
 def Ren.add (k : Nat) : Ren := ⟨(· + k)⟩
 
 @[simp]
@@ -32,6 +176,41 @@ theorem Ren.add_zero : add 0 = id := by simp [Ren.add, Ren.id]
 @[simp]
 theorem Ren.add_one : add 1 = succ := by simp [Ren.add, Ren.succ]
 
+def HetRen.add T (k : Nat) : HetRen T := ⟨(· + k)⟩
+
+@[simp]
+theorem HetRen.add_action {k x} : (add T k).act x = x + k := by simp [HetRen.add]
+
+@[simp]
+theorem HetRen.add_zero : add T 0 = id T := by simp [HetRen.add, HetRen.id]
+
+@[simp]
+theorem HetRen.add_one : add T 1 = succ T := by simp [HetRen.add, HetRen.succ]
+
+def Subst.add (k : Nat) : Subst S := ⟨λ x => re $ x + k⟩
+
+@[simp]
+theorem Subst.add_action {k x} : (@add S k).act x = re (x + k) := by simp [Subst.add]
+
+@[simp]
+theorem Subst.add_zero : @add S 0 = id := by simp [Subst.add, Subst.id]
+
+@[simp]
+theorem Subst.add_one : @add S 1 = succ := by simp [Subst.add, Subst.succ]
+
+def HetSubst.add (k : Nat) : HetSubst S T := ⟨λ x => re $ x + k⟩
+
+@[simp]
+theorem HetSubst.add_action {k x} : (@add S T k).act x = re (x + k) := by simp [HetSubst.add]
+
+@[simp]
+theorem HetSubst.add_zero : @add S T 0 = id T := by simp [HetSubst.add, HetSubst.id]
+
+@[simp]
+theorem HetSubst.add_one : @add S T 1 = succ T := by simp [HetSubst.add, HetSubst.succ]
+----------------------------------------------------------------------------------------------------
+---- Subtraction
+----------------------------------------------------------------------------------------------------
 def Ren.sub (k : Nat) : Ren := ⟨(· - k)⟩
 
 @[simp]
@@ -43,11 +222,23 @@ theorem Ren.sub_zero : sub 0 = id := by simp [Ren.sub, Ren.id]
 @[simp]
 theorem Ren.sub_one : sub 1 = pred := by simp [Ren.sub, Ren.pred]
 
+def HetRen.sub T (k : Nat) : HetRen T := ⟨(· - k)⟩
+
+@[simp]
+theorem HetRen.sub_action {k x} : (sub T k).act x = x - k := by simp [HetRen.sub]
+
+@[simp]
+theorem HetRen.sub_zero : sub T 0 = id T := by simp [HetRen.sub, HetRen.id]
+
+@[simp]
+theorem HetRen.sub_one : sub T 1 = pred T := by simp [HetRen.sub, HetRen.pred]
+----------------------------------------------------------------------------------------------------
+---- Cons
+----------------------------------------------------------------------------------------------------
 def Ren.cons (a : Nat) (r : Ren) : Ren := .mk λ n =>
   match n with
   | 0 => a
   | n + 1 => r.act n
-
 infixr:67 (name := Ren.cons_notation) " :: " => Ren.cons
 
 @[simp]
@@ -56,6 +247,46 @@ theorem Ren.cons_action0 {a} {r : Ren} : (a::r).act 0 = a := by simp [Ren.cons]
 @[simp]
 theorem Ren.cons_action {a i} {r : Ren} : (a::r).act (i + 1) = r.act i := by simp [Ren.cons]
 
+def HetRen.cons (a : Nat) (r : HetRen T) : HetRen T := .mk λ n =>
+  match n with
+  | 0 => a
+  | n + 1 => r.act n
+infixr:67 (name := HetRen.cons_notation) " :: " => HetRen.cons
+
+@[simp]
+theorem HetRen.cons_action0 {a} {r : HetRen T} : (a::r).act 0 = a := by simp [HetRen.cons]
+
+@[simp]
+theorem HetRen.cons_action {a i} {r : HetRen T} : (a::r).act (i + 1) = r.act i := by
+  simp [HetRen.cons]
+
+def Subst.cons (a : Action S) (r : Subst S) : Subst S := .mk λ n =>
+  match n with
+  | 0 => a
+  | n + 1 => r.act n
+infixr:67 (name := Subst.cons_notation) " :: " => Subst.cons
+
+@[simp]
+theorem Subst.cons_action0 {a} {r : Subst S} : (a::r).act 0 = a := by simp [Subst.cons]
+
+@[simp]
+theorem Subst.cons_action {a i} {r : Subst S} : (a::r).act (i + 1) = r.act i := by simp [Subst.cons]
+
+def HetSubst.cons (a : Action T) (r : HetSubst S T) : HetSubst S T := .mk λ n =>
+  match n with
+  | 0 => a
+  | n + 1 => r.act n
+infixr:67 (name := HetSubst.cons_notation) " :: " => HetSubst.cons
+
+@[simp]
+theorem HetSubst.cons_action0 {a} {r : HetSubst S T} : (a::r).act 0 = a := by simp [HetSubst.cons]
+
+@[simp]
+theorem HetSubst.cons_action {a i} {r : HetSubst S T} : (a::r).act (i + 1) = r.act i := by
+  simp [HetSubst.cons]
+----------------------------------------------------------------------------------------------------
+---- Append
+----------------------------------------------------------------------------------------------------
 def Ren.append : List Nat -> Ren -> Ren
 | .nil, r => r
 | .cons hd tl, r => hd::append tl r
@@ -79,7 +310,7 @@ theorem Ren.append_action_lt {r : Ren} {i}
   | 0 => rfl
   | i + 1 => append_action_lt (r := r) (ℓ := tl) (by grind)
 
-@[simp, grind =]
+@[simp, grind <-]
 theorem Ren.append_action_ge {r : Ren} {i}
   : {ℓ : List Nat} -> (h : i ≥ ℓ.length) -> (ℓ ++ r).act i = r.act (i - ℓ.length)
 | .nil, h => by simp
@@ -88,9 +319,107 @@ theorem Ren.append_action_ge {r : Ren} {i}
   | 0 => by simp at h
   | i + 1 => @append_action_ge r i tl (by grind) |> cast (by simp)
 
+def HetRen.append : List Nat -> HetRen T -> HetRen T
+| .nil, r => r
+| .cons hd tl, r => hd::append tl r
+
+instance : HAppend (List Nat) (HetRen T) (HetRen T) where
+  hAppend := HetRen.append
+
+@[simp]
+theorem HetRen.append_nil {r : HetRen T} : ([] : List Nat) ++ r = r := by
+  simp [HAppend.hAppend, HetRen.append]
+
+@[simp]
+theorem HetRen.append_cons {a} {ℓ : List Nat} {r : HetRen T} : (a::ℓ) ++ r = a::(ℓ ++ r) := by
+  simp [HAppend.hAppend, HetRen.append]
+
+@[simp, grind <-]
+theorem HetRen.append_action_lt {r : HetRen T} {i}
+  : {ℓ : List Nat} -> (h : i < ℓ.length) -> (ℓ ++ r).act i = ℓ[i]
+| .cons hd tl, h =>
+  match i with
+  | 0 => rfl
+  | i + 1 => append_action_lt (r := r) (ℓ := tl) (by grind)
+
+@[simp, grind <-]
+theorem HetRen.append_action_ge {r : HetRen T} {i}
+  : {ℓ : List Nat} -> (h : i ≥ ℓ.length) -> (ℓ ++ r).act i = r.act (i - ℓ.length)
+| .nil, h => by simp
+| .cons hd tl, h =>
+  match i with
+  | 0 => by simp at h
+  | i + 1 => @append_action_ge r i tl (by grind) |> cast (by simp)
+
+def Subst.append : List (Action S) -> Subst S -> Subst S
+| .nil, r => r
+| .cons hd tl, r => hd::append tl r
+
+instance : HAppend (List $ Action S) (Subst S) (Subst S) where
+  hAppend := Subst.append
+
+@[simp]
+theorem Subst.append_nil {r : Subst S} : ([] : List $ Action S) ++ r = r := by
+  simp [HAppend.hAppend, Subst.append]
+
+@[simp]
+theorem Subst.append_cons {a} {ℓ : List $ Action S} {r : Subst S} : (a::ℓ) ++ r = a::(ℓ ++ r) := by
+  simp [HAppend.hAppend, Subst.append]
+
+@[simp, grind <-]
+theorem Subst.append_action_lt {r : Subst S} {i}
+  : {ℓ : List $ Action S} -> (h : i < ℓ.length) -> (ℓ ++ r).act i = ℓ[i]
+| .cons hd tl, h =>
+  match i with
+  | 0 => rfl
+  | i + 1 => append_action_lt (r := r) (ℓ := tl) (by grind)
+
+@[simp, grind <-]
+theorem Subst.append_action_ge {r : Subst S} {i}
+  : {ℓ : List $ Action S} -> (h : i ≥ ℓ.length) -> (ℓ ++ r).act i = r.act (i - ℓ.length)
+| .nil, h => by simp
+| .cons hd tl, h =>
+  match i with
+  | 0 => by simp at h
+  | i + 1 => @append_action_ge r i tl (by grind) |> cast (by simp)
+
+def HetSubst.append : List (Action T) -> HetSubst S T -> HetSubst S T
+| .nil, r => r
+| .cons hd tl, r => hd::append tl r
+
+instance : HAppend (List $ Action T) (HetSubst S T) (HetSubst S T) where
+  hAppend := HetSubst.append
+
+@[simp]
+theorem HetSubst.append_nil {r : HetSubst S T} : ([] : List $ Action T) ++ r = r := by
+  simp [HAppend.hAppend, HetSubst.append]
+
+@[simp]
+theorem HetSubst.append_cons {a} {ℓ : List $ Action T} {r : HetSubst S T}
+  : (a::ℓ) ++ r = a::(ℓ ++ r)
+:= by simp [HAppend.hAppend, HetSubst.append]
+
+@[simp, grind <-]
+theorem HetSubst.append_action_lt {r : HetSubst S T} {i}
+  : {ℓ : List $ Action T} -> (h : i < ℓ.length) -> (ℓ ++ r).act i = ℓ[i]
+| .cons hd tl, h =>
+  match i with
+  | 0 => rfl
+  | i + 1 => append_action_lt (r := r) (ℓ := tl) (by grind)
+
+@[simp, grind <-]
+theorem HetSubst.append_action_ge {r : HetSubst S T} {i}
+  : {ℓ : List $ Action T} -> (h : i ≥ ℓ.length) -> (ℓ ++ r).act i = r.act (i - ℓ.length)
+| .nil, h => by simp
+| .cons hd tl, h =>
+  match i with
+  | 0 => by simp at h
+  | i + 1 => @append_action_ge r i tl (by grind) |> cast (by simp)
+----------------------------------------------------------------------------------------------------
+---- Composition
+----------------------------------------------------------------------------------------------------
 def Ren.compose : Ren -> Ren -> Ren
 | r1, r2 => .mk λ n => r2.act (r1.act n)
-
 infixr:85 (name := Ren.compose_notation) " ∘ " => Ren.compose
 
 @[simp]
@@ -109,6 +438,46 @@ theorem Ren.compose_id_right {r : Ren} : r ∘ id = r := by
 theorem Ren.compose_assoc {r1 r2 r3 : Ren} : (r1 ∘ r2) ∘ r3 = r1 ∘ r2 ∘ r3 := by
   simp [Ren.compose]
 
+def HetRen.compose : HetRen T -> HetRen T -> HetRen T
+| r1, r2 => .mk λ n => r2.act (r1.act n)
+infixr:85 (name := HetRen.compose_notation) " ∘ " => HetRen.compose
+
+@[simp]
+theorem HetRen.compose_action {r1 r2 : HetRen T} {x} : (r1 ∘ r2).act x = r2.act (r1.act x) := by
+  simp [HetRen.compose]
+
+@[simp]
+theorem HetRen.compose_id_left {r : HetRen T} : id T ∘ r = r := by
+  simp [HetRen.compose, HetRen.id]
+
+@[simp]
+theorem HetRen.compose_id_right {r : HetRen T} : r ∘ id T = r := by
+  simp [HetRen.compose, HetRen.id]
+
+@[simp]
+theorem HetRen.compose_assoc {r1 r2 r3 : HetRen T} : (r1 ∘ r2) ∘ r3 = r1 ∘ r2 ∘ r3 := by
+  simp [HetRen.compose]
+
+def Subst.compose [RenMap S] [SubstMap S] : Subst S -> Subst S -> Subst S
+| σ, τ => .mk λ n => (σ.act n)[τ.het _]
+infixr:85 (name := Subst.compose_notation) " ∘ " => Subst.compose
+
+@[simp]
+theorem Subst.compose_action [RenMap S] [SubstMap S] {σ τ : Subst S} {x}
+  : (σ ∘ τ).act x = (σ.act x)[τ.het _]
+:= by simp [Subst.compose]
+
+def HetSubst.compose [HetRenMap S T] [HetSubstMap S T] : HetSubst S T -> HetSubst S T -> HetSubst S T
+| σ, τ => .mk λ n => (σ.act n)[τ]
+infixr:85 (name := Subst.compose_notation) " ∘ " => Subst.compose
+
+@[simp]
+theorem Subst.compose_action [RenMap S] [SubstMap S] {σ τ : Subst S} {x}
+  : (σ ∘ τ).act x = (σ.act x)[τ.het _]
+:= by simp [Subst.compose]
+----------------------------------------------------------------------------------------------------
+---- Lift
+----------------------------------------------------------------------------------------------------
 def Ren.lift (r : Ren) (k : Nat := 1) : Ren := .mk λ n =>
   if n < k then n else r.act (n - k) + k
 
@@ -137,19 +506,19 @@ theorem Ren.lift_id {k} : Ren.lift Ren.id k = Ren.id := by
   simp [Ren.id, Ren.lift]; congr; funext; case _ x =>
   cases x <;> simp; omega
 
-theorem Ren.compose_lift_k1 {r1 r2 : Ren} : (r1 ∘ r2).lift = r1.lift ∘ r2.lift := by
+theorem Ren.lift_compose_k1 {r1 r2 : Ren} : (r1 ∘ r2).lift = r1.lift ∘ r2.lift := by
   simp [Ren.compose, Ren.lift]
   funext; case _ x =>
   cases x <;> simp
 
 @[simp]
-theorem Ren.compose_lift {k} {r1 r2 : Ren} : (r1 ∘ r2).lift k = r1.lift k ∘ r2.lift k := by
+theorem Ren.lift_compose {k} {r1 r2 : Ren} : (r1 ∘ r2).lift k = r1.lift k ∘ r2.lift k := by
   induction k generalizing r1 r2; simp
   case _ k ih =>
     rw [lift_of_succ, ih]
     rw [lift_of_succ (r := r1)]
     rw [lift_of_succ (r := r2)]
-    rw [compose_lift_k1]
+    rw [lift_compose_k1]
 
 
 
