LeanSubst/Types.lean
@@ -14,6 +14,11 @@ export RenMap (rmap)
 
 macro:max t:term noWs "⟨" r:term "⟩" : term => `(rmap $r $t)
 
+@[app_unexpander rmap]
+def unexpand_rmap : Lean.PrettyPrinter.Unexpander
+| `($_ $r $t) => `($t⟨$r⟩)
+| _ => throw ()
+
 structure HetRen (T : Type u2) where
   act : Nat -> Nat
 
@@ -22,27 +27,48 @@ class HetRenMap (S : Type u1) (T : Type u2) where
 
 export HetRenMap (hrmap)
 
-inductive Subst.Action (S : Type u1) where
-| re : Nat -> Subst.Action S
-| su : S -> Subst.Action S
+macro:max t:term noWs "⟨" r:term "⟩" : term => `(hrmap $r $t)
+
+@[app_unexpander rmap]
+def unexpand_hrmap : Lean.PrettyPrinter.Unexpander
+| `($_ $r $t) => `($t⟨$r⟩)
+| _ => throw ()
+
+inductive Action (S : Type u1) where
+| re : Nat -> Action S
+| su : S -> Action S
 deriving Repr
 
-export Subst.Action (re su)
+export Action (re su)
 
 structure Subst (S : Type u1) where
-  act : Nat -> Subst.Action S
+  act : Nat -> Action S
 
 class SubstMap (S : Type u1) where
   smap : Subst S -> S -> S
 
 export SubstMap (smap)
 
+macro:max t:term noWs "[" σ:term "]" : term => `(smap $σ $t)
+
+@[app_unexpander smap]
+def unexpand_smap : Lean.PrettyPrinter.Unexpander
+| `($_ $σ $t) => `($t[$σ])
+| _ => throw ()
+
 structure HetSubst (S : Type u1) (T : Type u2) where
-  act : Nat -> Subst.Action S
+  act : Nat -> Action T
 
 class HetSubstMap (S : Type u1) (T : Type u2) where
   hsmap : HetSubst S T -> S -> S
 
 export HetSubstMap (hsmap)
+
+macro:max t:term noWs "[" σ:term "]" : term => `(hsmap $σ $t)
+
+@[app_unexpander smap]
+def unexpand_hsmap : Lean.PrettyPrinter.Unexpander
+| `($_ $σ $t) => `($t[$σ])
+| _ => throw ()
 
 end LeanSubst
